footprint.dfy
@@ -1,0 +1,29 @@
+module Footprint {
+  type pos = x: int | x > 0 witness 1
+
+  trait {:termination false} footprintable<M> {
+    ghost opaque const ReprDepth: pos
+
+    ghost function ReprFamily(n: nat): set<object>
+      decreases n
+      ensures n > 0 ==>
+        ReprFamily(n) >= ReprFamily(n-1)
+      reads this, if n == 0 then {} else ReprFamily(n-1)
+    ghost function Repr(): set<object>
+      reads this, ReprFamily(ReprDepth-1)
+    {
+      ReprFamily(ReprDepth)
+    }
+
+    lemma ReprLemma()
+      ensures Repr() == ReprFamily(ReprDepth)
+    {}
+
+    ghost predicate Valid()
+      reads this, Repr()
+
+    ghost function Model(): M
+      reads this, Repr()
+      requires Valid()
+  }
+}
